DataflowToMinimp/Translation.v
@@ -8,6 +8,9 @@ Require Import Rustre.Dataflow.Memories.
 Require Import List.
 Require Import Coq.Lists.List.
 Import List.ListNotations.
+Require Import Coq.Sorting.Permutation.
+Require Import Morphisms.
+
 Open Scope positive.
 Open Scope list.
 
@@ -37,7 +40,8 @@ Module Type TRANSLATION
        (Import Op    : OPERATORS)
        (Import OpAux : OPERATORS_AUX Op)
        (Import SynDF : Rustre.Dataflow.Syntax.SYNTAX Ids Op)
-       (Import SynMP : Rustre.Minimp.Syntax.SYNTAX Ids Op OpAux).
+       (Import SynMP : Rustre.Minimp.Syntax.SYNTAX Ids Op OpAux)
+       (Import Mem   : MEMORIES Ids Op SynDF).
 
   (* definition is needed in signature *)
   Definition gather_eq
@@ -171,25 +175,407 @@ Module Type TRANSLATION
       constructor; auto.
       constructor; auto.
   Qed.
+
+  (** Properties of translation functions *)
+
+  Instance eq_equiv : Equivalence PS.eq.
+  Proof. firstorder. Qed.
+
+  Instance List_fold_left_add_Proper (xs: list ident) :
+    Proper (PS.eq ==> PS.eq)
+           (List.fold_left (fun s i => PS.add i s) xs).
+  Proof.
+    induction xs as [|x xs IH]; intros S S' Heq; [exact Heq|].
+    assert (PS.eq (PS.add x S) (PS.add x S')) as Heq'
+        by (rewrite Heq; reflexivity).
+    simpl; rewrite Heq'; reflexivity.
+  Qed.
+
+  Instance List_fold_left_memory_eq_Proper (eqs: list equation) :
+    Proper (PS.eq ==> PS.eq)
+           (List.fold_left memory_eq eqs).
+  Proof.
+    induction eqs as [|eq eqs IH]; intros S S' Heq; [exact Heq|].
+    simpl.
+    apply IH.
+    destruct eq; [apply Heq|apply Heq|].
+    simpl; rewrite Heq; reflexivity.
+  Qed.
+
+  Lemma add_ps_from_list_cons:
+    forall xs x, PS.eq (PS.add x (ps_from_list xs))
+                  (ps_from_list (x::xs)).
+  Proof.
+    intros; unfold ps_from_list; simpl.
+    generalize PS.empty as S.
+    induction xs as [|y xs IH]; [ reflexivity | ].
+    intro S; simpl; rewrite IH; rewrite PSP.add_add; reflexivity.
+  Qed.
+
+  Lemma ps_from_list_gather_eqs_memories:
+    forall eqs, PS.eq (ps_from_list (fst (gather_eqs eqs))) (memories eqs).
+  Proof.
+    induction eqs as [|eq eqs IH]; [reflexivity|].
+    unfold memories, gather_eqs.
+    assert (forall eqs F S,
+               PS.eq (ps_from_list (fst (List.fold_left gather_eq eqs (F, S))))
+                     (List.fold_left memory_eq eqs (ps_from_list F))) as HH.
+    { clear eq eqs IH; induction eqs as [|eq eqs IH]; [reflexivity|].
+      intros F S.
+      destruct eq; [now apply IH|now apply IH|].
+      simpl; rewrite IH; rewrite add_ps_from_list_cons; reflexivity. }
+    rewrite HH; reflexivity.
+  Qed.
+
+  Instance tovar_Proper :
+    Proper (PS.eq ==> eq ==> eq) tovar.
+  Proof.
+    intros M M' HMeq x x' Hxeq; rewrite <- Hxeq; clear Hxeq x'.
+    unfold tovar; destruct x as [x ty].
+    destruct (PS.mem x M) eqn:Hmem;
+      rewrite <- HMeq, Hmem; reflexivity.
+  Qed.
+
+  Instance translate_lexp_Proper :
+    Proper (PS.eq ==> eq ==> eq) translate_lexp.
+  Proof.
+    intros M M' HMeq e e' Heq; rewrite <- Heq; clear Heq e'.
+    revert M M' HMeq.
+    induction e (* using lexp_ind2 *); intros M M' HMeq; simpl; auto.
+    + rewrite HMeq; auto.
+    + f_equal; auto.
+    + f_equal; auto.
+  Qed.
+
+  Instance translate_cexp_Proper :
+    Proper (PS.eq ==> eq ==> eq ==> eq) translate_cexp.
+  Proof.
+    intros M M' HMeq y y' Hyeq c c' Hceq; rewrite <- Hyeq, <- Hceq;
+    clear y' c' Hyeq Hceq.
+    revert M M' HMeq.
+    induction c; intros; simpl.
+    - erewrite IHc1; try eassumption.
+      erewrite IHc2; try eassumption. 
+      rewrite HMeq; auto.
+    - erewrite IHc1; try eassumption.
+      erewrite IHc2; try eassumption. 
+      rewrite HMeq; auto.
+    - rewrite HMeq; auto.
+  Qed.
+
+  Instance Control_Proper :
+    Proper (PS.eq ==> eq ==> eq ==> eq) Control.
+  Proof.
+    intros M M' HMeq ck ck' Hckeq e e' Heq; rewrite <-Hckeq, <-Heq;
+    clear ck' e' Hckeq Heq.
+    revert e; induction ck as [ |ck' IH s sv].
+    - reflexivity.
+    - intro e.
+      destruct sv; simpl; rewrite IH, HMeq; reflexivity.
+  Qed.
+
+  Instance translate_eqn_Proper :
+    Proper (PS.eq ==> eq ==> eq) translate_eqn.
+  Proof.
+    intros M M' HMeq eq eq' Heq; rewrite <- Heq; clear Heq eq'.
+    destruct eq as [y ck []|y ck f []|y ck v0 []]; simpl; try now rewrite HMeq.
+    - rewrite HMeq at 1 2. do 3 f_equal.
+      apply List.map_ext. intro. now rewrite HMeq.
+  Qed.
+
+  Instance translate_eqns_Proper :
+    Proper (PS.eq ==> eq ==> eq) translate_eqns.
+  Proof.
+    intros M M' Heq eqs eqs' Heqs.
+    rewrite <- Heqs; clear Heqs.
+    unfold translate_eqns.
+    assert (forall S S',
+               S = S' ->
+               List.fold_left (fun i eq => Comp (translate_eqn M eq) i) eqs S
+               = List.fold_left (fun i eq => Comp (translate_eqn M' eq) i) eqs S')
+      as HH.
+    { revert M M' Heq.
+      induction eqs as [|eq eqs IH]; intros M M' Heq S S' HSeq; [apply HSeq|].
+      simpl; apply IH with (1:=Heq); rewrite HSeq, Heq; reflexivity. }
+    rewrite HH with (S':=Skip); reflexivity.
+  Qed.
   
-(*
-  Lemma blah:
+  Lemma permutation_partition:
+    forall {A:Type} p (l: list A),
+      Permutation l (fst (partition p l) ++ snd (partition p l)).
+  Proof.
+    induction l as [|x l].
+    now constructor.
+    simpl.
+    destruct (p x).
+    - rewrite (surjective_pairing (partition _ _)).
+      now simpl; apply Permutation_cons.
+    - rewrite (surjective_pairing (partition _ _)).
+      now simpl; apply Permutation_cons_app.
+  Qed.
+
+  Lemma Permutation_app_assoc:
+    forall {A: Type} (ws: list A) xs ys,
+      Permutation ((ws ++ xs) ++ ys) (ws ++ xs ++ ys).
+  Proof.
+    intros.
+    induction ws.
+    reflexivity.
+    now apply Permutation_cons.
+  Qed.
+
+  Instance InMembers_Permutation_Proper (A B:Type):
+    Proper (eq ==> Permutation (A:=A * B) ==> iff) InMembers.
+  Proof.
+    intros x y Heq xs ys Hperm.
+    rewrite Heq. clear Heq x.
+    split; intro Hinm.
+    - apply InMembers_In in Hinm.
+      destruct Hinm as [b Hinm].
+      apply Permutation_in with (2:=Hinm) in Hperm.
+      apply In_InMembers with (1:=Hperm).
+    - apply InMembers_In in Hinm.
+      destruct Hinm as [b Hinm].
+      symmetry in Hperm.
+      apply Permutation_in with (2:=Hinm) in Hperm.
+      apply In_InMembers with (1:=Hperm).
+  Qed.
+
+  Instance NoDupMembers_Permutation_Proper (A B:Type):
+    Proper (Permutation (A:=A * B) ==> iff) NoDupMembers.
+  Proof.
+    intros xs ys Hperm.
+    induction Hperm.
+    - now intuition.
+    - destruct x as [x y].
+      rewrite 2 nodupmembers_cons, IHHperm, Hperm.
+      reflexivity.
+    - split; intro HH.
+      + inversion HH as [|a b l' Hninm Hndup]. clear HH. subst.
+        destruct x as [x y].
+        inversion Hndup as [|c d l' Hinm' Hndup']. clear Hndup. subst.
+        econstructor.
+        * intro Hinm. apply Hinm'.
+          inversion_clear Hinm; subst; auto.
+          exfalso; apply Hninm. now constructor.
+        * constructor; auto. intro Hinm.
+          apply Hninm. constructor (assumption).
+      + inversion HH as [|a b l' Hninm Hndup]. clear HH. subst.
+        destruct y as [x y].
+        inversion Hndup as [|c d l' Hinm' Hndup']. clear Hndup. subst.
+        econstructor.
+        * intro Hinm. apply Hinm'.
+          inversion_clear Hinm; subst; auto.
+          exfalso; apply Hninm. now constructor.
+        * constructor; auto. intro Hinm.
+          apply Hninm. constructor (assumption).
+    - now rewrite IHHperm1.
+  Qed.
+
+  Lemma NoDup_cons:
+    forall {A} (x:A) xs,
+      NoDup (x::xs) <-> ~In x xs /\ NoDup xs.
+  Proof.
+    split; intro HH.
+    - inversion_clear HH. intuition.
+    - destruct HH. constructor; auto.
+  Qed.
+
+  Instance In_Permutation_Proper (A:Type):
+    Proper (eq ==> Permutation (A:=A) ==> iff) (@In A).
+  Proof.
+    intros x y Hxy xs ys Hperm.
+    subst y.
+    split; intro HH; [|symmetry in Hperm];
+      now apply Permutation_in with (1:=Hperm) in HH.
+  Qed.
+  
+  Instance NoDup_Permutation_Proper (A:Type):
+    Proper (Permutation (A:=A) ==> iff) (@NoDup A).
+  Proof.
+    intros xs ys Hperm.
+    induction Hperm.
+    - now intuition.
+    - rewrite 2 NoDup_cons, IHHperm, Hperm.
+      reflexivity.
+    - split; inversion_clear 1 as [|? ? Hnin Hndup];
+        inversion_clear Hndup as [|? ? Hnin' Hndup'];
+        (constructor; [|constructor]); auto; intro Hnin3;
+          apply Hnin.
+      + inversion Hnin3; [|contradiction].
+        subst. now constructor.
+      + constructor (assumption).
+      + inversion Hnin3; [|contradiction].
+        subst. now constructor.
+      + constructor (assumption).
+    - now rewrite IHHperm1, IHHperm2.
+  Qed.
+  
+  Lemma Permutation_Forall:
+    forall {A} (l l': list A) P,
+      Permutation l l' ->
+      Forall P l ->
+      Forall P l'.
+  Proof.
+    induction 1; inversion 1; auto.
+    match goal with H:Forall _ (_ :: _) |- _ => inversion H end.
+    repeat constructor; auto.
+  Qed.
+
+  Instance Forall_Permutation_Proper (A:Type):
+    Proper (eq ==> Permutation (A:=A) ==> iff) Forall.
+  Proof.
+    intros P Q HPQ xs ys Hperm.
+    subst P.
+    split; intro HH; [|symmetry in Hperm];
+      apply Permutation_Forall with (1:=Hperm) (2:=HH).
+  Qed.
+
+  Lemma Forall_app_weaken:
+    forall {A} xs P (ys : list A),
+      Forall P (xs ++ ys) ->
+      Forall P ys.
+  Proof.
+    intros ** HH. apply Forall_app in HH. intuition.
+  Qed.
+
+  Lemma partition_switch:
+    forall {A} f g,
+      (forall x:A, f x = g x) ->
+      forall xs, partition f xs = partition g xs.
+  Proof.
+    intros ** Hfg xs.
+    induction xs as [|x xs]; auto. simpl.
+    specialize (Hfg x). symmetry in Hfg. rewrite Hfg, IHxs.
+    reflexivity.
+  Qed.
+
+  Lemma partition_filter:
+    forall {A} P (xs: list A),
+      Permutation (fst (partition P xs)) (filter P xs).
+  Proof.
+    induction xs as [|x xs]; auto.
+    simpl; rewrite (surjective_pairing (partition P xs)).
+    destruct (P x); auto.
+    now apply Permutation_cons.
+  Qed.
+
+  Definition is_fby (eq: equation) : bool :=
+    match eq with
+    | EqFby _ _ _ _ => true
+    | _ => false
+    end.
+
+  Definition is_app (eq: equation) : bool :=
+    match eq with
+    | EqApp _ _ _ _ _ => true
+    | _ => false
+    end.
+
+  Definition is_def (eq: equation) : bool :=
+    match eq with
+    | EqDef _ _ _ => true
+    | _ => false
+    end.
+
+  Lemma is_filtered_eqs:
     forall eqs,
-      MemsDeclared (fst_gather_eqs eqs) (reset_method eqs).(m_body).
+      Permutation
+        (filter is_def eqs ++ filter is_app eqs ++ filter is_fby eqs)
+        eqs.
+  Proof.
+    induction eqs as [|eq eqs]; auto.
+    destruct eq; simpl.
+    - now apply Permutation_cons.
+    - rewrite <-Permutation_cons_app.
+      apply Permutation_cons; reflexivity.
+      now symmetry.
+    - symmetry.
+      rewrite <-Permutation_app_assoc.
+      apply Permutation_cons_app.
+      rewrite Permutation_app_assoc.
+      now symmetry.
+  Qed.
 
-
-    (* TODO: MemsDeclared mems (reset_method eqns).(m_body) *)
-    (* TODO: InstanceDeclared objs (reset_method eqns).(m_body) *)
-
-    (* TODO: Then tackle the trickier step method *)
- *)
+  Lemma NoDup_app_weaken:
+    forall {A} (xs: list A) ys,
+      NoDup (xs ++ ys) ->
+      NoDup xs.
+  Proof.
+    Hint Constructors NoDup.
+    intros ** Hndup.
+    induction xs as [|x xs]; auto.
+    inversion_clear Hndup as [|? ? Hnin Hndup'].
+    apply IHxs in Hndup'.
+    constructor; auto.
+    intro Hin. apply Hnin.
+    apply in_or_app; now left.
+  Qed.
   
+  Lemma fst_partition_memories_var_defined:
+    forall n,
+      map fst (fst (partition
+                      (fun x=> PS.mem (fst x) (memories n.(n_eqs))) n.(n_vars)))
+      = map var_defined (filter is_fby n.(n_eqs)).
+  Proof.
+  Admitted.
+
+  Lemma fst_gather_eqs_var_defined:
+    forall n,
+      map fst (snd (gather_eqs n.(n_eqs)))
+      = map var_defined (filter is_app n.(n_eqs)).
+  Proof.
+  Admitted.
+  
+  Lemma VarsDeclared_translate_eqns:
+    forall n mems,
+      VarsDeclared
+        (snd (partition (fun x=> PS.mem (fst x) mems) n.(n_vars))
+         ++ [n.(n_out)])
+        (translate_eqns mems n.(n_eqs)).
+  Proof.
+  Admitted.
+
+  Lemma MemsDeclared_translate_eqns:
+    forall n mems,
+      MemsDeclared
+        (fst (partition (fun x=> PS.mem (fst x) mems) n.(n_vars)))
+        (translate_eqns mems n.(n_eqs)).
+  Proof.
+  Admitted.
+
+  Lemma MemsDeclared_translate_reset_eqns:
+    forall n mems,
+      MemsDeclared
+        (fst (partition (fun x=> PS.mem (fst x) mems) n.(n_vars)))
+        (translate_reset_eqns n.(n_eqs)).
+  Proof.
+  Admitted.
+
+  Lemma InstanceDeclared_translate_eqns:
+    forall n,
+      InstanceDeclared (snd (gather_eqs n.(n_eqs)))
+        (translate_eqns (ps_from_list (fst (gather_eqs n.(n_eqs)))) n.(n_eqs)).
+  Proof.
+  Admitted.
+
+  Lemma InstanceDeclared_translate_reset_eqns:
+    forall n,
+      InstanceDeclared (snd (gather_eqs n.(n_eqs)))
+                       (translate_reset_eqns n.(n_eqs)).
+  Proof.
+  Admitted.
+
   (* =translate_node= *)
   (* definition is needed in signature *)
   Program Definition translate_node (n: node) : class :=
-    let (memids, dobjs) := gather_eqs n.(n_eqs) in
+    let gathered := gather_eqs n.(n_eqs) in
+    let memids := fst gathered in
+    let dobjs := snd gathered in
     let mems := ps_from_list memids in
-    let (dmems, dvars) := partition (fun x=>PS.mem (fst x) mems) n.(n_vars) in
+    let partitioned := partition (fun x=>PS.mem (fst x) mems) n.(n_vars) in
+    let dmems := fst partitioned in
+    let dvars := snd partitioned in
     {| c_name    := n.(n_name);
        c_mems    := dmems;
        c_objs    := dobjs;
@@ -203,56 +589,135 @@ Module Type TRANSLATION
                          m_good      := _
                       |};
                       reset_method n.(n_eqs) ];
-       c_nodupmems := _;
-       c_nodupobjs := _;
+       c_nodups   := _;
        
        c_memsdecl := _;
        c_instdecl := _
     |}.
   (* =end= *)
   Next Obligation.
-  Admitted.
+    repeat progress match goal with
+                    | H: (_ , _) = _ |- _ =>
+                      rewrite surjective_pairing in H;
+                        injection H; clear H
+                    end.
+    intros; subst.
+    rewrite (Permutation_app_comm n.(n_in)).
+    rewrite Permutation_app_assoc.
+    match goal with |- context [snd (partition ?p ?l)] =>
+      apply (NoDupMembers_app_r (fst (partition p l))) end.
+    match goal with |- NoDupMembers ?l =>
+      cut (Permutation l (n_in n ++ n_vars n ++ [n_out n]))
+    end.
+    intro Hperm; rewrite Hperm. now apply n_nodup.
+    assert (Permutation (n.(n_in) ++ n.(n_vars) ++ [n.(n_out)])
+                        (n.(n_vars) ++ [n.(n_out)] ++ n.(n_in))) as Hr
+        by (now rewrite Permutation_app_comm, Permutation_app_assoc).
+    rewrite Hr.
+    rewrite <- (Permutation_app_assoc _ _ ([n.(n_out)] ++ n.(n_in))).
+    apply Permutation_app; auto.
+    symmetry; apply permutation_partition.
+  Qed.
   Next Obligation.
-  Admitted.
+    repeat progress match goal with
+                    | H: (_ , _) = _ |- _ =>
+                      rewrite surjective_pairing in H;
+                        injection H; clear H
+                    end.
+    intros; subst.
+    now apply VarsDeclared_translate_eqns.
+  Qed.
   Next Obligation.
-  Admitted.
+    repeat progress match goal with
+                    | H: (_ , _) = _ |- _ =>
+                      rewrite surjective_pairing in H;
+                        injection H; clear H
+                    end.
+    intros; subst.
+    rewrite (Permutation_app_comm n.(n_in)).
+    rewrite Permutation_app_assoc.
+    match goal with |- context [snd (partition ?p ?l)] =>
+      apply (Forall_app_weaken (fst (partition p l))) end.
+    match goal with |- Forall _ ?l =>
+      cut (Permutation l (n_in n ++ n_vars n ++ [n_out n]))
+    end.
+    intro Hperm; rewrite Hperm. now apply n_good.
+    assert (Permutation (n.(n_in) ++ n.(n_vars) ++ [n.(n_out)])
+                        (n.(n_vars) ++ [n.(n_out)] ++ n.(n_in))) as Hr
+        by (now rewrite Permutation_app_comm, Permutation_app_assoc).
+    rewrite Hr.
+    rewrite <- (Permutation_app_assoc _ _ ([n.(n_out)] ++ n.(n_in))).
+    apply Permutation_app; auto.
+    symmetry; apply permutation_partition.
+  Qed.
   Next Obligation.
-  Admitted.
+    repeat progress match goal with
+                    | H: (_ , _) = _ |- _ =>
+                      rewrite surjective_pairing in H;
+                        injection H; clear H
+                    end.
+    intros; subst.
+    rewrite partition_switch
+    with (g:=fun x=> PS.mem (fst x) (memories n.(n_eqs))).
+    2:intro x; now rewrite ps_from_list_gather_eqs_memories.
+    rewrite fst_partition_memories_var_defined.
+    rewrite fst_gather_eqs_var_defined.
+    eapply (NoDup_app_weaken _ (map var_defined (filter is_def n.(n_eqs)))).
+    rewrite Permutation_app_comm.
+    (* Annoying, Coq should be able to rewrite these directly... *)
+    match goal with |- NoDup (?l1 ++ ?l2 ++ ?l3) =>
+      assert (Permutation (l1 ++ l2 ++ l3) (l1 ++ l3 ++ l2)) as Hperm
+        by (rewrite Permutation_app'; auto; now rewrite Permutation_app_comm)
+    end.
+    rewrite Hperm. clear Hperm.
+    rewrite <- 2 map_app.
+    match goal with |- NoDup (map ?f ?l) =>
+      assert (Permutation (map f l) (map f n.(n_eqs))) as Hperm
+        by (apply Permutation_map_aux; apply is_filtered_eqs)
+    end.
+    rewrite Hperm. clear Hperm.
+    rewrite n_defd.
+    apply fst_NoDupMembers.
+    apply NoDupMembers_app_r with (ws:=n.(n_in)).
+    apply n_nodup.
+  Qed.
   Next Obligation.
-  Admitted.
+    repeat constructor;
+      simpl;
+      repeat progress match goal with
+                      | H: (_ , _) = _ |- _ =>
+                        rewrite surjective_pairing in H;
+                          injection H; clear H
+                      end;
+      intros; subst.
+      now apply MemsDeclared_translate_eqns.
+      now apply MemsDeclared_translate_reset_eqns.
+  Qed.       
   Next Obligation.
-  Admitted.
-  Next Obligation.
-  Admitted.
+    repeat constructor;
+      simpl;
+      repeat progress match goal with
+                      | H: (_ , _) = _ |- _ =>
+                        rewrite surjective_pairing in H;
+                          injection H; clear H
+                      end;
+      intros; subst.
+    now apply InstanceDeclared_translate_eqns.
+    now apply InstanceDeclared_translate_reset_eqns.
+  Qed.
 
   (* =translate= *)
   (* definition is needed in signature *)
   Definition translate (G: global) : program :=
     List.map translate_node G.
   (* =end= *)
-    
-  Lemma translate_node_name:
-    forall n, (translate_node n).(c_name) = n.(n_name).
-  Proof.
-    destruct n.
-    unfold translate_node.
-    simpl.
-    (* TODO: There must be a better way! *)
-    destruct (gather_eqs n_eqs0).
-    destruct (partition (fun x => PS.mem (fst x) (ps_from_list l)) n_vars0).
-    reflexivity.
-  Qed.
-  
+
   Lemma exists_step_method:
     forall node,
     exists stepm,
       find_method step (translate_node node).(c_methods) = Some stepm.
   Proof.
     intro node.
-    unfold translate_node.
-    destruct (gather_eqs node.(n_eqs)).
-    destruct (partition (fun x => PS.mem (fst x) (ps_from_list l))
-                        node.(n_vars)).
     simpl. rewrite ident_eqb_refl. eauto.
   Qed.
 
@@ -262,15 +727,10 @@ Module Type TRANSLATION
       = Some (reset_method node.(n_eqs)).
   Proof.
     intro node.
-    unfold translate_node.
-    destruct (gather_eqs node.(n_eqs)).
-    destruct (partition (fun x => PS.mem (fst x) (ps_from_list l))
-                        node.(n_vars)).
-    simpl.
     assert (ident_eqb step reset = false) as Hsr.
     apply ident_eqb_neq.
     apply PositiveOrder.neq_sym. apply reset_not_step.
-    now rewrite Hsr, ident_eqb_refl.
+    simpl. now rewrite Hsr, ident_eqb_refl.
   Qed.
 
   Lemma find_method_stepm:
@@ -279,40 +739,30 @@ Module Type TRANSLATION
       stepm.(m_out) = [node.(n_out)].
   Proof.
     intros node stepm.
-    unfold translate_node.
-    destruct (gather_eqs node.(n_eqs)).
-    destruct (partition (fun x => PS.mem (fst x) (ps_from_list l))
-                        node.(n_vars)).
     simpl. rewrite ident_eqb_refl.
     injection 1.
     intro HH; rewrite <-HH.
     reflexivity.
   Qed.
-  
-  (* (** ** Properties *) *)
 
-  (* Lemma ps_from_list_pre_spec: *)
-  (*   forall x l S, (List.In x l \/ PS.In x S) *)
-  (*            <-> *)
-  (*            PS.In x (List.fold_left (fun s i=>PS.add i s) l S). *)
-  (* Proof. *)
-  (*   induction l as [|l ls IH]. *)
-  (*   - firstorder. *)
-  (*   - split; intro HH. *)
-  (*     + firstorder. *)
-  (*     + apply IH in HH. *)
-  (*       destruct HH as [HH|HH]; try apply PS.add_spec in HH; firstorder. *)
-  (* Qed. *)
-
-  (* Lemma ps_from_list_spec: *)
-  (*   forall x l, List.In x l <-> PS.In x (ps_from_list l). *)
-  (* Proof. *)
-  (*   unfold ps_from_list. *)
-  (*   intros. *)
-  (*   rewrite <- ps_from_list_pre_spec with (S:=PS.empty). *)
-  (*   split; try intros [H | H]; try tauto. *)
-  (*   apply not_In_empty in H; contradiction. *)
-  (* Qed. *)
+  Lemma find_class_translate:
+    forall n G cls prog',
+      find_class n (translate G) = Some (cls, prog')
+      -> (exists node, find_node n G = Some node
+                       /\ cls = translate_node node).
+  Proof.
+    induction G as [|node G]; [now inversion 1|].
+    intros ** Hfind.
+    simpl in Hfind.
+    destruct (equiv_dec node.(n_name) n) as [Heq|Hneq].
+    - rewrite Heq, ident_eqb_refl in Hfind.
+      injection Hfind; intros; subst.
+      exists node. split; auto.
+      simpl. now rewrite Heq, ident_eqb_refl.
+    - apply ident_eqb_neq in Hneq. rewrite Hneq in Hfind.
+      apply IHG in Hfind. destruct Hfind as (node' & Hfind & Hcls).
+      exists node'. simpl. rewrite Hneq. auto.
+  Qed.
   
 End TRANSLATION.
 
@@ -322,9 +772,10 @@ Module TranslationFun
        (Import OpAux: OPERATORS_AUX Op)
        (Import SynDF : Rustre.Dataflow.Syntax.SYNTAX Ids Op)
        (Import SynMP : Rustre.Minimp.Syntax.SYNTAX Ids Op OpAux)
-       <: TRANSLATION Ids Op OpAux SynDF SynMP.
+       (Import Mem : MEMORIES Ids Op SynDF)
+       <: TRANSLATION Ids Op OpAux SynDF SynMP Mem.
 
-  Include TRANSLATION Ids Op OpAux SynDF SynMP. 
+  Include TRANSLATION Ids Op OpAux SynDF SynMP Mem.
   
 End TranslationFun.
 
