Dataflow/Semantics.v
@@ -1,6 +1,7 @@
 Require Import List.
 Import List.ListNotations.
 Open Scope list_scope.
+Require Import Coq.Sorting.Permutation.
 
 Require Import Coq.FSets.FMapPositive.
 Require Import Rustre.Common.
@@ -297,9 +298,10 @@ environment.
 
   with sem_node G: ident -> stream (list value) -> stream value -> Prop :=
        | SNode:
-           forall bk f xss ys i o v eqs ingt0 decl nodup good,
+           forall bk f xss ys i o v eqs ingt0 defd decl nodup good,
              clock_of xss bk ->
-             find_node f G = Some (mk_node f i o v eqs ingt0 decl nodup good) ->
+             find_node f G = Some (mk_node f i o v eqs
+                                           ingt0 defd decl nodup good) ->
              (exists H,
                  sem_vars bk H (map fst i) xss
                  /\ sem_var bk H (fst o) ys
@@ -378,12 +380,14 @@ enough: it does not support the internal fixpoint introduced by
              (v     : list (ident * typ))
              (eqs   : list equation)
              (ingt0 : 0 < length i)
+             (defd  : Permutation (map var_defined eqs)
+                                  (map fst (v ++ [o])))
              (decl  : Forall (VarsDeclared (i ++ v ++ [o])) eqs)
              (nodup : NoDupMembers (i ++ v ++ [o]))
              (good  : Forall NotReserved (i ++ v ++ [o]))
              (Hck   : clock_of xss bk)
              (Hf    : find_node f G =
-                      Some (mk_node f i o v eqs ingt0 decl nodup good))
+                      Some (mk_node f i o v eqs ingt0 defd decl nodup good))
              (Heqs  : exists H,
             sem_vars bk H (map fst i) xss
             /\ sem_var bk H (fst o) ys
@@ -395,7 +399,8 @@ enough: it does not support the internal fixpoint introduced by
             /\ (forall n, absent_list xss n <-> ys n = absent)
             /\ Forall (fun eq=> exists Hsem, P bk H eq Hsem) eqs)
         -> Pn f xss ys
-              (SNode G bk f xss ys i o v eqs ingt0 decl nodup good Hck Hf Heqs).
+              (SNode G bk f xss ys i o v eqs ingt0
+                     defd decl nodup good Hck Hf Heqs).
 
     Fixpoint sem_equation_mult (bk: stream bool)
              (H  : history)
@@ -416,8 +421,10 @@ enough: it does not support the internal fixpoint introduced by
                        (ys : stream value)
                        (Hn : sem_node G f ls ys) {struct Hn} : Pn f ls ys Hn :=
            match Hn in (sem_node _ f ls ys) return (Pn f ls ys Hn) with
-           | SNode bk f ls ys i o v eqs ingt0 decl nodup good Hck Hf Hnode =>
-             SNode_case bk f ls ys i o v eqs ingt0 decl nodup good Hck Hf Hnode
+           | SNode bk f ls ys i o v eqs
+                   ingt0 defd decl nodup good Hck Hf Hnode =>
+             SNode_case bk f ls ys i o v eqs
+                        ingt0 defd decl nodup good Hck Hf Hnode
                         (* Turn: exists H : history,
                         (forall n, sem_var H (v_name i) n (xs n))
                      /\ (forall n, sem_var H (v_name o) n (ys n))
@@ -804,7 +811,7 @@ clock to [sem_var_instant] too. *)
     induction Hsem as [
          | bk H y ck f lae ls ys ty Hlae Hvar Hnode IH
          |
-         | bk f xs ys i o v eqs ingt0 decl nodup good Hbk Hf Heqs IH]
+         | bk f xs ys i o v eqs ingt0 defd decl nodup good Hbk Hf Heqs IH]
             using sem_node_mult
           with (P := fun bk H eq Hsem => ~Is_node_in_eq node.(n_name) eq
                                       -> sem_equation G bk H eq).
@@ -820,15 +827,16 @@ clock to [sem_var_instant] too. *)
       destruct IH as [H [Hxs [Hys [Hout Heqs]]]].
       exists H.
       repeat (split; eauto).
-      set (cnode := {| n_name   := f;
-                       n_in     := i;
-                       n_out    := o;
-                       n_vars   := v;
-                       n_eqs    := eqs;
-                       n_ingt0  := ingt0;
-                       n_decl   := decl;
-                       n_nodup  := nodup;
-                       n_good   := good
+      set (cnode := {| n_name  := f;
+                       n_in    := i;
+                       n_out   := o;
+                       n_vars  := v;
+                       n_eqs   := eqs;
+                       n_ingt0 := ingt0;
+                       n_defd  := defd;
+                       n_decl  := decl;
+                       n_nodup := nodup;
+                       n_good  := good
                     |}).
       assert (Forall (fun eq => ~ Is_node_in_eq (n_name node) eq) (n_eqs cnode))
         by (eapply Is_node_in_Forall; try eassumption;
@@ -840,16 +848,17 @@ clock to [sem_var_instant] too. *)
   Qed.
 
   Lemma find_node_find_again:
-    forall G f i o v eqs ingt0 decl nodup good g,
+    forall G f i o v eqs ingt0 defd decl nodup good g,
       Ordered_nodes G
       -> find_node f G =
          Some {| n_name := f; n_in := i;    n_out := o;
                  n_vars := v; n_eqs := eqs; n_decl := decl;
-                 n_ingt0 := ingt0; n_nodup := nodup; n_good := good |}
+                 n_ingt0 := ingt0; n_defd := defd; n_nodup := nodup;
+                 n_good := good |}
       -> Is_node_in g eqs
       -> Exists (fun nd=> g = nd.(n_name)) G.
   Proof.
-    intros G f i o v eqs ingt0 decl nodup good g Hord Hfind Hini.
+    intros G f i o v eqs ingt0 defd decl nodup good g Hord Hfind Hini.
     apply find_node_split in Hfind.
     destruct Hfind as [bG [aG Hfind]].
     rewrite Hfind in *.
@@ -876,7 +885,7 @@ clock to [sem_var_instant] too. *)
     induction Hsem as [
        | bk H y f lae ls ys Hlae Hvar Hnode IH
        |
-       | bk f xs ys i o v eqs ingt0 decl nodup good Hbk Hfind Heqs IH]
+       | bk f xs ys i o v eqs ingt0 defd decl nodup good Hbk Hfind Heqs IH]
           using sem_node_mult
         with (P := fun bk H eq Hsem =>
                      ~Is_node_in_eq nd.(n_name) eq
@@ -911,7 +920,7 @@ clock to [sem_var_instant] too. *)
                    Is_node_in_eq g eq
                    -> Exists (fun nd=> g = nd.(n_name)) G) eqs) as HH.
     {
-      clear decl nodup good Hfind Heqs Hnf.
+      clear defd decl nodup good Hfind Heqs Hnf.
       induction eqs as [|eq eqs IH]; [now constructor|].
       constructor.
       - intros g Hini.
